core/TofinoPipeline.v
@@ -96,4 +96,101 @@ Section SWITCH.
       egress_pipe st2 p st3 p' ->
       process_egress_packets st1 (enque p ps) st3 (enque p' ps').
 
+  Definition process_queue_form {A: Type} (q: queue A) : Prop :=
+    match q with
+    | empty_queue => True
+    | nonempty_queue front _ _ => front = []
+    end.
+
+  Lemma process_egress_packets_input_form: forall st1 qin st2 qout,
+      process_ingress_packets st1 qin st2 qout -> process_queue_form qin.
+  Proof.
+    intros. induction H; simpl; auto. rename IHprocess_ingress_packets into IH.
+    destruct ps; simpl in *; auto.
+  Qed.
+
+  Lemma process_queue_form_enque: forall {A: Type} (a: A) q,
+      process_queue_form q -> process_queue_form (enque a q).
+  Proof. intros. destruct q; simpl in *; auto. Qed.
+
+  Lemma process_queue_form_enque_inv: forall {A: Type} (a: A) q,
+        process_queue_form (enque a q) -> process_queue_form q.
+  Proof. intros. destruct q; simpl in *; auto. Qed.
+
+  Lemma process_queue_form_split: forall {A: Type} (q: queue A),
+      process_queue_form q ->
+      forall i, 0 <= i <= qlength q ->
+           exists q1 q2, qlength q1 = i /\ q = concat_queue q1 q2 /\
+                      process_queue_form q1 /\ process_queue_form q2.
+  Proof.
+    intros. rewrite qlength_eq, Zlength_correct in H0. remember (length (list_rep q)) as n.
+    revert dependent q. revert dependent n. induction n; intros.
+    - assert (i = 0) by lia. subst i. destruct q.
+      2: simpl in Heqn; rewrite app_length in Heqn; simpl in Heqn; lia.
+      exists empty_queue, empty_queue. simpl. auto.
+    - destruct q. 1: simpl in Heqn; discriminate. simpl in H. subst. simpl in Heqn.
+      rewrite rev'_eq, rev_length in Heqn. inversion Heqn. clear Heqn. destruct l0.
+      + simpl in H1. subst n. assert (i = 0 \/ i = 1) by lia. destruct H; subst i.
+        * exists empty_queue, (nonempty_queue [] a []). simpl. auto.
+        * exists (nonempty_queue [] a []), empty_queue. simpl. auto.
+      + rename l0 into l. rename a0 into b. destruct (Z_le_lt_dec i (Z.of_nat n)).
+        * specialize (IHn ltac:(lia) (nonempty_queue [] a l) ltac:(reflexivity)).
+          simpl in H1, IHn. rewrite rev'_eq, rev_length in IHn. specialize (IHn H1).
+          destruct IHn as (q1 & q2 & ? & ? & ? & ?). exists q1, (enque b q2).
+          split; [|split; [|split]]; auto. 2: apply process_queue_form_enque; assumption.
+          destruct q1, q2; simpl in *; subst; try discriminate; inversion H2; reflexivity.
+        * assert (i = Z.of_nat (S n)) by lia. subst i. simpl in H1.
+          exists (nonempty_queue [] a (b :: l)), empty_queue. split; [|simpl; auto].
+          simpl qlength. rewrite Zlength_correct. simpl length. lia.
+  Qed.
+
+  Lemma enque_eq_concat_form: forall {A: Type} (p: A) ps q1 q2,
+      enque p ps = concat_queue q1 q2 -> q2 <> empty_queue -> process_queue_form q2 ->
+      exists q3, ps = concat_queue q1 q3 /\ process_queue_form q3 /\ q2 = enque p q3.
+  Proof.
+    intros. destruct q2. 1: contradiction. simpl in H1. subst. clear H0.
+    destruct q1, ps; simpl in H; inversion H; subst; simpl.
+    - exists empty_queue. simpl. auto.
+    - exists (nonempty_queue [] a l1). simpl. auto.
+    - assert (length (l0 ++ a :: l1) = length (l0 ++ a :: l1)) by reflexivity.
+      rewrite <- H3 in H0 at 1. rewrite app_length in H0. simpl in H0. lia.
+    - destruct l0.
+      + simpl in H3. inversion H3. subst. exists empty_queue. simpl. auto.
+      + rewrite <- app_comm_cons in H3. inversion H3. subst. clear H3 H.
+        exists (nonempty_queue [] a l0). simpl. auto.
+  Qed.
+
+  Lemma process_ingress_packets_split: forall st1 qin st2 qout,
+      process_ingress_packets st1 qin st2 qout ->
+      forall len, 0 <= len <= qlength qin ->
+             exists q1 q2 q3 q4 st3,
+               qlength q1 = len /\
+                 qin = concat_queue q1 q2 /\
+                 qout = concat_queue q3 q4 /\
+                 process_ingress_packets st1 q1 st3 q3 /\
+                 process_ingress_packets st3 q2 st2 q4.
+  Proof.
+    intros. pose proof (process_egress_packets_input_form _ _ _ _ H).
+    destruct (process_queue_form_split _ H1 _ H0) as [q1 [q2 [? [? [? ?]]]]].
+    exists q1, q2. revert dependent q2. revert dependent q1. induction H; intros.
+    - exists empty_queue, empty_queue, st. symmetry in H3. apply concat_queue_eq_empty in H3.
+      destruct H3. subst. do 4 (split; auto); constructor.
+    - rename IHprocess_ingress_packets into IH. destruct (Z_le_gt_dec len (qlength ps)).
+      + specialize (IH ltac:(lia) (process_queue_form_enque_inv _ _ H1) _ H3 H4).
+        destruct (empty_queue_dec q2).
+        1: subst; rewrite concat_queue_empty in H5; subst q1; rewrite qlength_enque in l; lia.
+        destruct (enque_eq_concat_form _ _ _ _ H5 n H6) as [q3 [? [? ?]]]. specialize (IH _ H7 H8).
+        destruct IH as (q4 & q5 & st4 & ? & ? & ? & ? & ?).
+        exists q4, (concat_queue q5 (traffic_manager md p')), st4. subst ps'.
+        rewrite concat_queue_assoc. do 4 (split; auto). subst q2. econstructor; eauto.
+      + rewrite qlength_enque in H0. assert (len = qlength ps + 1) by lia. clear g H0 IH.
+        pose proof (@eq_refl _ (qlength (enque p ps))). rewrite H5 in H0 at 1.
+        rewrite qlength_concat, qlength_enque in H0. assert (qlength q2 = 0) by lia.
+        rewrite qlength_0_iff in H8. subst q2. rewrite concat_queue_empty in *.
+        exists (concat_queue ps' (traffic_manager md p')), empty_queue, st3.
+        rewrite concat_queue_empty. subst q1. do 4 (split; auto).
+        * econstructor; eauto.
+        * constructor.
+  Qed.
+
 End SWITCH.
